Wrote up unifiable types

02Typed/Typechecking.thy
@@ -24,62 +24,62 @@ primrec typecheck' :: "subst \<Rightarrow> var set \<Rightarrow> 'a expr\<^sub>s
     where
   "typecheck' \<Gamma> vs (Var\<^sub>s x) = (case \<Gamma> x of 
       Some t \<Rightarrow> (Var\<^sub>s x, t, vs, []) 
-    | None \<Rightarrow> (Var\<^sub>s x, Ctor ''Num'' [], vs, fail))"
-| "typecheck' \<Gamma> vs (Const\<^sub>s k) = (Const\<^sub>s k, Ctor ''Num'' [], vs, [])"
+    | None \<Rightarrow> (Var\<^sub>s x, Num\<^sub>\<tau>, vs, fail))"
+| "typecheck' \<Gamma> vs (Const\<^sub>s k) = (Const\<^sub>s k, Num\<^sub>\<tau>, vs, [])"
 | "typecheck' \<Gamma> vs (Lam\<^sub>s x t e) = (
     let v = fresh vs
     in let (e', t, vs', con) = typecheck' (\<Gamma>(x \<mapsto> Var v)) (insert v vs) e
-    in (Lam\<^sub>s x (Var v) e', Ctor ''Arrow'' [Var v, t], vs', con))"
+    in (Lam\<^sub>s x (Var v) e', Arrow\<^sub>\<tau> (Var v) t, vs', con))"
 | "typecheck' \<Gamma> vs (App\<^sub>s e\<^sub>1 e\<^sub>2) = (
     let v = fresh vs
     in let (e\<^sub>1', t\<^sub>1, vs', con\<^sub>1) = typecheck' \<Gamma> (insert v vs) e\<^sub>1 
     in let (e\<^sub>2', t\<^sub>2, vs'', con\<^sub>2) = typecheck' \<Gamma> vs' e\<^sub>2 
-    in (App\<^sub>s e\<^sub>1' e\<^sub>2', Var v, vs'', con\<^sub>1 @ con\<^sub>2 @ [(t\<^sub>1, Ctor ''Arrow'' [t\<^sub>2, Var v])]))"
+    in (App\<^sub>s e\<^sub>1' e\<^sub>2', Var v, vs'', con\<^sub>1 @ con\<^sub>2 @ [(t\<^sub>1, Arrow\<^sub>\<tau> t\<^sub>2 (Var v))]))"
 
 primrec solidify :: "uterm expr\<^sub>s \<Rightarrow> ty expr\<^sub>s" where
   "solidify (Var\<^sub>s x) = Var\<^sub>s x"
 | "solidify (Const\<^sub>s k) = Const\<^sub>s k"
-| "solidify (Lam\<^sub>s x t e) = Lam\<^sub>s x (typeify t) (solidify e)"
+| "solidify (Lam\<^sub>s x t e) = Lam\<^sub>s x (to_type t) (solidify e)"
 | "solidify (App\<^sub>s e\<^sub>1 e\<^sub>2) = App\<^sub>s (solidify e\<^sub>1) (solidify e\<^sub>2)"
 
 primrec liquify :: "ty expr\<^sub>s \<Rightarrow> uterm expr\<^sub>s" where
   "liquify (Var\<^sub>s x) = Var\<^sub>s x"
 | "liquify (Const\<^sub>s k) = Const\<^sub>s k"
-| "liquify (Lam\<^sub>s x t e) = Lam\<^sub>s x (untypeify t) (liquify e)"
+| "liquify (Lam\<^sub>s x t e) = Lam\<^sub>s x (to_unifiable t) (liquify e)"
 | "liquify (App\<^sub>s e\<^sub>1 e\<^sub>2) = App\<^sub>s (liquify e\<^sub>1) (liquify e\<^sub>2)"
 
 primrec partial_solidify :: "var set \<Rightarrow> uterm expr\<^sub>s \<Rightarrow> uterm expr\<^sub>s" where
   "partial_solidify vs (Var\<^sub>s x) = Var\<^sub>s x"
 | "partial_solidify vs (Const\<^sub>s k) = Const\<^sub>s k"
-| "partial_solidify vs (Lam\<^sub>s x t e) = Lam\<^sub>s x (partial_typeify vs t) (partial_solidify vs e)"
+| "partial_solidify vs (Lam\<^sub>s x t e) = Lam\<^sub>s x (eliminate_vars vs t) (partial_solidify vs e)"
 | "partial_solidify vs (App\<^sub>s e\<^sub>1 e\<^sub>2) = App\<^sub>s (partial_solidify vs e\<^sub>1) (partial_solidify vs e\<^sub>2)"
 
 fun typecheck :: "'a expr\<^sub>s \<rightharpoonup> ty expr\<^sub>s \<times> ty" where
   "typecheck e = (
     let (e', t, vs, con) = typecheck' Map.empty {} e
     in case unify con of 
-        Some sub \<Rightarrow> Some (solidify (hsubst sub e'), typeify (subst sub t))
+        Some sub \<Rightarrow> Some (solidify (hsubst sub e'), to_type (subst sub t))
       | None \<Rightarrow> None)"
 
 primrec valid_ty_hexpr :: "uterm expr\<^sub>s \<Rightarrow> bool" where
   "valid_ty_hexpr (Var\<^sub>s x) = True"
 | "valid_ty_hexpr (Const\<^sub>s k) = True"
-| "valid_ty_hexpr (Lam\<^sub>s x t e) = (valid_ty_uexpr t \<and> valid_ty_hexpr e)"
+| "valid_ty_hexpr (Lam\<^sub>s x t e) = (valid_ty_term t \<and> valid_ty_hexpr e)"
 | "valid_ty_hexpr (App\<^sub>s e\<^sub>1 e\<^sub>2) = (valid_ty_hexpr e\<^sub>1 \<and> valid_ty_hexpr e\<^sub>2)"
 
 lemma typecheck_induct [consumes 1, case_names Var\<^sub>sS Var\<^sub>sN Const\<^sub>s Lam\<^sub>s App\<^sub>s]: "
   typecheck' \<Gamma> vs e = (e', t, vs', con) \<Longrightarrow> 
   (\<And>\<Gamma> vs t x. \<Gamma> x = Some t \<Longrightarrow> P \<Gamma> vs (Var\<^sub>s x) (Var\<^sub>s x) t vs []) \<Longrightarrow> 
-  (\<And>\<Gamma> vs x. \<Gamma> x = None \<Longrightarrow> P \<Gamma> vs (Var\<^sub>s x) (Var\<^sub>s x) (Ctor ''Num'' [])  vs fail) \<Longrightarrow> 
-  (\<And>\<Gamma> vs k. P \<Gamma> vs (Const\<^sub>s k) (Const\<^sub>s k) (Ctor ''Num'' []) vs []) \<Longrightarrow> 
+  (\<And>\<Gamma> vs x. \<Gamma> x = None \<Longrightarrow> P \<Gamma> vs (Var\<^sub>s x) (Var\<^sub>s x) Num\<^sub>\<tau> vs fail) \<Longrightarrow> 
+  (\<And>\<Gamma> vs k. P \<Gamma> vs (Const\<^sub>s k) (Const\<^sub>s k) Num\<^sub>\<tau> vs []) \<Longrightarrow> 
   (\<And>\<Gamma> vs vs' con x u e\<^sub>1 e\<^sub>1' t' v. v = fresh vs \<Longrightarrow> typecheck' (\<Gamma>(x \<mapsto> Var v)) (insert v vs) e\<^sub>1 = 
     (e\<^sub>1', t', vs', con) \<Longrightarrow> P (\<Gamma>(x \<mapsto> Var v)) (insert v vs) e\<^sub>1 e\<^sub>1' t' vs' con \<Longrightarrow> 
-      P \<Gamma> vs (Lam\<^sub>s x u e\<^sub>1) (Lam\<^sub>s x (Var v) e\<^sub>1') (Ctor ''Arrow'' [Var v, t']) vs' con) \<Longrightarrow> 
+      P \<Gamma> vs (Lam\<^sub>s x u e\<^sub>1) (Lam\<^sub>s x (Var v) e\<^sub>1') (Arrow\<^sub>\<tau> (Var v) t') vs' con) \<Longrightarrow> 
   (\<And>\<Gamma> vs vs' e\<^sub>1 e\<^sub>2 v e\<^sub>1' t\<^sub>1 vs'' con\<^sub>1 e\<^sub>2' t\<^sub>2 con\<^sub>2. v = fresh vs \<Longrightarrow> 
     typecheck' \<Gamma> (insert v vs) e\<^sub>1 = (e\<^sub>1', t\<^sub>1, vs'', con\<^sub>1) \<Longrightarrow> 
       typecheck' \<Gamma> vs'' e\<^sub>2 = (e\<^sub>2', t\<^sub>2, vs', con\<^sub>2) \<Longrightarrow> P \<Gamma> (insert v vs) e\<^sub>1 e\<^sub>1' t\<^sub>1 vs'' con\<^sub>1 \<Longrightarrow> 
         P \<Gamma> vs'' e\<^sub>2 e\<^sub>2' t\<^sub>2 vs' con\<^sub>2 \<Longrightarrow> P \<Gamma> vs (App\<^sub>s e\<^sub>1 e\<^sub>2) (App\<^sub>s e\<^sub>1' e\<^sub>2') (Var v) vs' 
-          (con\<^sub>1 @ con\<^sub>2 @ [(t\<^sub>1, Ctor ''Arrow'' [t\<^sub>2, Var v])])) \<Longrightarrow> 
+          (con\<^sub>1 @ con\<^sub>2 @ [(t\<^sub>1, Arrow\<^sub>\<tau> t\<^sub>2 (Var v))])) \<Longrightarrow> 
     P \<Gamma> vs e e' t vs' con"
   by (induction e arbitrary: \<Gamma> vs e' t vs' con) 
      (auto simp add: Let_def split: option.splits prod.splits)
@@ -128,7 +128,7 @@ qed auto
 lemma [simp]: "hsubst (combine_subst s t) e = hsubst s (hsubst t e)"
   by (induction e) simp_all
 
-lemma [elim]: "typecheck' \<Gamma> vs e = (e', t, vs', con) \<Longrightarrow> valid_ty_subst \<Gamma> \<Longrightarrow> valid_ty_uexpr t"
+lemma [elim]: "typecheck' \<Gamma> vs e = (e', t, vs', con) \<Longrightarrow> valid_ty_subst \<Gamma> \<Longrightarrow> valid_ty_term t"
   by (induction rule: typecheck_induct) auto
 
 lemma [elim]: "typecheck' \<Gamma> vs e = (e', t, vs', con) \<Longrightarrow> valid_ty_subst \<Gamma> \<Longrightarrow> valid_ty_hexpr e'"
@@ -136,36 +136,36 @@ lemma [elim]: "typecheck' \<Gamma> vs e = (e', t, vs', con) \<Longrightarrow> va
 
 lemma typecheck_succeeds [simp]: "typecheck' \<Gamma> vs e = (e', t, vs', con) \<Longrightarrow> 
   valid_ty_subst \<Gamma> \<Longrightarrow> unify con = Some sub' \<Longrightarrow> sub specializes sub' \<Longrightarrow>
-    map_option (typeify \<circ> subst sub) \<circ> \<Gamma> \<turnstile>\<^sub>t solidify (hsubst sub e') : typeify (subst sub t)"
+    map_option (to_type \<circ> subst sub) \<circ> \<Gamma> \<turnstile>\<^sub>t solidify (hsubst sub e') : to_type (subst sub t)"
 proof (induction arbitrary: sub' rule: typecheck_induct)
   case (Var\<^sub>sS \<Gamma> vs t x)
   thus ?case by simp
 next
   case (Lam\<^sub>s \<Gamma> vs vs' con x u e\<^sub>1 e\<^sub>1' t' v)
   hence "valid_ty_subst (\<Gamma>(x \<mapsto> Var v))" by simp
-  with Lam\<^sub>s have "map_option (typeify \<circ> subst sub) \<circ> \<Gamma>(x \<mapsto> Var v) \<turnstile>\<^sub>t solidify (hsubst sub e\<^sub>1') : 
-      typeify (subst sub t')" by blast
-  hence "map_option (typeify \<circ> subst sub) \<circ> \<Gamma> \<turnstile>\<^sub>t solidify (hsubst sub (Lam\<^sub>s x (Var v) e\<^sub>1')) :
-    typeify (subst sub (Ctor ''Arrow'' [Var v, t']))" by simp
+  with Lam\<^sub>s have "map_option (to_type \<circ> subst sub) \<circ> \<Gamma>(x \<mapsto> Var v) \<turnstile>\<^sub>t solidify (hsubst sub e\<^sub>1') : 
+      to_type (subst sub t')" by blast
+  hence "map_option (to_type \<circ> subst sub) \<circ> \<Gamma> \<turnstile>\<^sub>t solidify (hsubst sub (Lam\<^sub>s x (Var v) e\<^sub>1')) :
+    to_type (subst sub (Arrow\<^sub>\<tau> (Var v) t'))" by simp
   thus ?case by blast
 next
   case (App\<^sub>s \<Gamma> vs vs' e\<^sub>1 e\<^sub>2 v e\<^sub>1' t\<^sub>1 vs'' con\<^sub>1 e\<^sub>2' t\<^sub>2 con\<^sub>2)
   then obtain s\<^sub>2 where S2: "unify (con\<^sub>1 @ con\<^sub>2) = Some s\<^sub>2 \<and> sub' specializes s\<^sub>2" by fastforce
   then obtain s\<^sub>3 where S3: "unify con\<^sub>1 = Some s\<^sub>3 \<and> s\<^sub>2 specializes s\<^sub>3" by fastforce
   with App\<^sub>s S2 have "sub specializes s\<^sub>3" by auto
-  with App\<^sub>s S2 S3 have T: "map_option (typeify \<circ> subst sub) \<circ> \<Gamma> \<turnstile>\<^sub>t solidify (hsubst sub e\<^sub>1') : 
-    typeify (subst sub t\<^sub>1)" by blast
-  from App\<^sub>s have "sub' unifies\<^sub>\<kappa> (con\<^sub>1 @ con\<^sub>2 @ [(t\<^sub>1, Ctor ''Arrow'' [t\<^sub>2, Var v])])" 
+  with App\<^sub>s S2 S3 have T: "map_option (to_type \<circ> subst sub) \<circ> \<Gamma> \<turnstile>\<^sub>t solidify (hsubst sub e\<^sub>1') : 
+    to_type (subst sub t\<^sub>1)" by blast
+  from App\<^sub>s have "sub' unifies\<^sub>\<kappa> (con\<^sub>1 @ con\<^sub>2 @ [(t\<^sub>1, Arrow\<^sub>\<tau> t\<^sub>2 (Var v))])" 
     by (metis unify_some) 
-  hence "sub' unifies t\<^sub>1 and Ctor ''Arrow'' [t\<^sub>2, Var v]" by simp
-  with App\<^sub>s have X: "sub unifies t\<^sub>1 and Ctor ''Arrow'' [t\<^sub>2, Var v]" by fastforce
+  hence "sub' unifies t\<^sub>1 and Arrow\<^sub>\<tau> t\<^sub>2 (Var v)" by simp
+  with App\<^sub>s have X: "sub unifies t\<^sub>1 and Arrow\<^sub>\<tau> t\<^sub>2 (Var v)" by fastforce
   from S2 obtain s\<^sub>4 where S4: "unify con\<^sub>2 = Some s\<^sub>4 \<and> s\<^sub>2 specializes s\<^sub>4" 
     using unify_append_snd by blast
   with App\<^sub>s S2 have "sub specializes s\<^sub>4" by auto
-  with App\<^sub>s S4 have "map_option (typeify \<circ> subst sub) \<circ> \<Gamma> \<turnstile>\<^sub>t solidify (hsubst sub e\<^sub>2') : 
-    typeify (subst sub t\<^sub>2)" by blast
-  with T X have "map_option (typeify \<circ> subst sub) \<circ> \<Gamma> \<turnstile>\<^sub>t solidify (hsubst sub (App\<^sub>s e\<^sub>1' e\<^sub>2')) : 
-    typeify (subst sub (Var v))" by simp
+  with App\<^sub>s S4 have "map_option (to_type \<circ> subst sub) \<circ> \<Gamma> \<turnstile>\<^sub>t solidify (hsubst sub e\<^sub>2') : 
+    to_type (subst sub t\<^sub>2)" by blast
+  with T X have "map_option (to_type \<circ> subst sub) \<circ> \<Gamma> \<turnstile>\<^sub>t solidify (hsubst sub (App\<^sub>s e\<^sub>1' e\<^sub>2')) : 
+    to_type (subst sub (Var v))" by simp
   thus ?case by blast
 qed simp_all
 
@@ -173,11 +173,11 @@ lemma [simp]: "typecheck e = Some (e\<^sub>t, t) \<Longrightarrow> Map.empty \<t
 proof -
   assume "typecheck e = Some (e\<^sub>t, t)"
   then obtain e' tt vs con sub where T: "typecheck' Map.empty {} e = (e', tt, vs, con) \<and>
-    unify con = Some sub \<and> e\<^sub>t = solidify (hsubst sub e') \<and> t = typeify (subst sub tt)" 
+    unify con = Some sub \<and> e\<^sub>t = solidify (hsubst sub e') \<and> t = to_type (subst sub tt)" 
       by (auto split: option.splits prod.splits)
-  moreover hence "map_option (typeify \<circ> subst sub) \<circ> Map.empty \<turnstile>\<^sub>t solidify (hsubst sub e') : 
-    typeify (subst sub tt)" by (metis typecheck_succeeds valid_empty specializes_refl)
-  moreover from T have "valid_ty_uexpr tt" and "valid_ty_hexpr e'" by auto
+  moreover hence "map_option (to_type \<circ> subst sub) \<circ> Map.empty \<turnstile>\<^sub>t solidify (hsubst sub e') : 
+    to_type (subst sub tt)" by (metis typecheck_succeeds valid_empty_subst specializes_refl)
+  moreover from T have "valid_ty_term tt" and "valid_ty_hexpr e'" by auto
   ultimately show "Map.empty \<turnstile>\<^sub>t e\<^sub>t : t" by simp
 qed
 
@@ -307,7 +307,7 @@ next
   show ?case
   proof (cases "x = z")
     case True
-    from T Lam\<^sub>s(2) have E: "e' = Lam\<^sub>s z (Var ?v) e'' \<and> tt = Ctor ''Arrow'' [Var ?v, tt'] \<and> 
+    from T Lam\<^sub>s(2) have E: "e' = Lam\<^sub>s z (Var ?v) e'' \<and> tt = Arrow\<^sub>\<tau> (Var ?v) tt' \<and> 
       vs'' = vs' \<and> con' = con" by (simp only: typecheck'.simps Let_def split: prod.splits) simp
     from T True E have T': "typecheck' (\<Gamma>(z \<mapsto> Var ?v)) (insert ?v vs) e = (e'', tt', vs', con)" 
       by simp
@@ -320,7 +320,7 @@ next
   next
     case False
     from Lam\<^sub>s have "typecheck' (\<Gamma>(x \<mapsto> Var y)) vs (Lam\<^sub>s z u e) = (e', tt, vs', con)" by blast
-    with T have E: "e' = Lam\<^sub>s z (Var ?v) e'' \<and> tt = Ctor ''Arrow'' [Var ?v, tt'] \<and> vs'' = vs' \<and> 
+    with T have E: "e' = Lam\<^sub>s z (Var ?v) e'' \<and> tt = Arrow\<^sub>\<tau> (Var ?v) tt' \<and> vs'' = vs' \<and> 
       con' = con" by (simp add: Let_def)
     from E T False have X: "typecheck' (\<Gamma>(z \<mapsto> Var ?v, x \<mapsto> Var y)) (insert ?v vs) e = 
       (e'', tt', vs', con)" by (metis fun_upd_twist)
@@ -345,7 +345,7 @@ next
     (e\<^sub>2', t\<^sub>2, vs''', con\<^sub>2)" by (metis prod_cases4)
   moreover from App\<^sub>s have "typecheck' (\<Gamma>(x \<mapsto> Var y)) vs (App\<^sub>s e1 e2) = (e', tt, vs', con)" by blast
   ultimately have E: "e' = App\<^sub>s e\<^sub>1' e\<^sub>2' \<and> tt = Var ?v \<and> vs''' = vs' \<and> 
-    con = con\<^sub>1 @ con\<^sub>2 @ [(t\<^sub>1, Ctor ''Arrow'' [t\<^sub>2, Var ?v])]" by (auto simp add: Let_def)
+    con = con\<^sub>1 @ con\<^sub>2 @ [(t\<^sub>1, Arrow\<^sub>\<tau> t\<^sub>2 (Var ?v))]" by (auto simp add: Let_def)
   from T1 have V: "vs \<subseteq> vs''" using vars_expand by blast
   from App\<^sub>s V have A: "y \<in> vs''" by auto
   from App\<^sub>s V have B: "subst_vars \<Gamma> \<subseteq> vs'' - {y}" by auto
@@ -360,73 +360,73 @@ next
   thus ?case by blast
 qed auto
 
-lemma typecheck_fails' [simp]: "map_option typeify \<circ> \<Gamma> \<turnstile>\<^sub>t e\<^sub>t : t \<Longrightarrow> finite vs \<Longrightarrow> 
+lemma typecheck_fails' [simp]: "map_option to_type \<circ> \<Gamma> \<turnstile>\<^sub>t e\<^sub>t : t \<Longrightarrow> finite vs \<Longrightarrow> 
   subst_vars \<Gamma> \<subseteq> vs \<Longrightarrow> valid_ty_subst \<Gamma> \<Longrightarrow> typecheck' \<Gamma> vs (erase e\<^sub>t) = (e', tt, vs', con) \<Longrightarrow> 
   \<exists>s. partial_solidify vs (hsubst s e') = liquify e\<^sub>t \<and> 
-  partial_typeify vs (subst s tt) = untypeify t \<and> dom s = vs' - vs \<and> 
-  subst_vars s = {} \<and> s unifies\<^sub>\<kappa> partial_typeify_constr vs con \<and> valid_ty_subst s \<and> idempotent s"
-proof (induction "map_option typeify \<circ> \<Gamma>" e\<^sub>t t arbitrary: \<Gamma> vs e' tt vs' con rule: typing\<^sub>t.induct)
+  eliminate_vars vs (subst s tt) = to_unifiable t \<and> dom s = vs' - vs \<and> 
+  subst_vars s = {} \<and> s unifies\<^sub>\<kappa> eliminate_vars_constr vs con \<and> valid_ty_subst s \<and> idempotent s"
+proof (induction "map_option to_type \<circ> \<Gamma>" e\<^sub>t t arbitrary: \<Gamma> vs e' tt vs' con rule: typing\<^sub>t.induct)
   case (tc\<^sub>t_lam x t\<^sub>1 e t\<^sub>2)
   let ?v = "fresh vs"
   obtain e'' t' vs'' con' where T: "typecheck' (\<Gamma>(x \<mapsto> Var ?v)) (insert ?v vs) (erase e) = 
     (e'', t', vs'', con')" by (metis prod_cases4)
-  with tc\<^sub>t_lam have E: "e' = Lam\<^sub>s x (Var ?v) e'' \<and> tt = Ctor ''Arrow'' [Var ?v, t'] \<and> vs'' = vs' \<and> 
+  with tc\<^sub>t_lam have E: "e' = Lam\<^sub>s x (Var ?v) e'' \<and> tt = Arrow\<^sub>\<tau> (Var ?v) t' \<and> vs'' = vs' \<and> 
     con' = con" by (simp add: Let_def)
   from tc\<^sub>t_lam have "subst_vars \<Gamma> \<subseteq> insert ?v vs" by auto
-  hence X: "subst_vars (\<Gamma>(x \<mapsto> untypeify t\<^sub>1)) \<subseteq> insert ?v vs" by simp
-  have Y: "(map_option typeify \<circ> \<Gamma>)(x \<mapsto> t\<^sub>1) = map_option typeify \<circ> (\<Gamma>(x \<mapsto> untypeify t\<^sub>1))" by simp
-  from tc\<^sub>t_lam have Z: "valid_ty_subst (\<Gamma>(x \<mapsto> untypeify t\<^sub>1))" by simp
-  from tc\<^sub>t_lam T have TC: "typecheck' (\<Gamma>(x \<mapsto> untypeify t\<^sub>1)) (insert ?v vs) (erase e) = 
-    (hsubst [?v \<mapsto> untypeify t\<^sub>1] e'', subst [?v \<mapsto> untypeify t\<^sub>1] t', vs'', 
-     constr_subst ?v (untypeify t\<^sub>1) con')" by simp
+  hence X: "subst_vars (\<Gamma>(x \<mapsto> to_unifiable t\<^sub>1)) \<subseteq> insert ?v vs" by simp
+  have Y: "(map_option to_type \<circ> \<Gamma>)(x \<mapsto> t\<^sub>1) = map_option to_type \<circ> (\<Gamma>(x \<mapsto> to_unifiable t\<^sub>1))" by simp
+  from tc\<^sub>t_lam have Z: "valid_ty_subst (\<Gamma>(x \<mapsto> to_unifiable t\<^sub>1))" by simp
+  from tc\<^sub>t_lam T have TC: "typecheck' (\<Gamma>(x \<mapsto> to_unifiable t\<^sub>1)) (insert ?v vs) (erase e) = 
+    (hsubst [?v \<mapsto> to_unifiable t\<^sub>1] e'', subst [?v \<mapsto> to_unifiable t\<^sub>1] t', vs'', 
+     constr_subst ?v (to_unifiable t\<^sub>1) con')" by simp
   from tc\<^sub>t_lam have "finite (insert ?v vs)" by simp
   with tc\<^sub>t_lam X Y Z TC obtain s where S: "
-    partial_solidify (insert ?v vs) (hsubst s (hsubst [?v \<mapsto> untypeify t\<^sub>1] e'')) = liquify e \<and> 
-    partial_typeify (insert ?v vs) (subst s (subst [?v \<mapsto> untypeify t\<^sub>1] t')) = untypeify t\<^sub>2 \<and>
-    s unifies\<^sub>\<kappa> partial_typeify_constr (insert ?v vs) (constr_subst ?v (untypeify t\<^sub>1) con') \<and> 
+    partial_solidify (insert ?v vs) (hsubst s (hsubst [?v \<mapsto> to_unifiable t\<^sub>1] e'')) = liquify e \<and> 
+    eliminate_vars (insert ?v vs) (subst s (subst [?v \<mapsto> to_unifiable t\<^sub>1] t')) = to_unifiable t\<^sub>2 \<and>
+    s unifies\<^sub>\<kappa> eliminate_vars_constr (insert ?v vs) (constr_subst ?v (to_unifiable t\<^sub>1) con') \<and> 
     dom s = vs'' - insert ?v vs \<and> subst_vars s = {} \<and> valid_ty_subst s \<and> idempotent s" by meson
-  from tc\<^sub>t_lam have "subst_vars (\<Gamma>(x \<mapsto> untypeify t\<^sub>1)) \<subseteq> vs" by simp
+  from tc\<^sub>t_lam have "subst_vars (\<Gamma>(x \<mapsto> to_unifiable t\<^sub>1)) \<subseteq> vs" by simp
   moreover from tc\<^sub>t_lam have FV: "?v \<notin> vs" by simp
-  ultimately have "?v \<notin> subst_vars (\<Gamma>(x \<mapsto> untypeify t\<^sub>1))" by blast
-  with tc\<^sub>t_lam TC have VCS: "?v \<notin> constr_vars (constr_subst ?v (untypeify t\<^sub>1) con')" by simp
-  have "htvars (hsubst [?v \<mapsto> untypeify t\<^sub>1] e') \<subseteq> 
-    htvars e' - dom [?v \<mapsto> untypeify t\<^sub>1] \<union> subst_vars [?v \<mapsto> untypeify t\<^sub>1]" 
+  ultimately have "?v \<notin> subst_vars (\<Gamma>(x \<mapsto> to_unifiable t\<^sub>1))" by blast
+  with tc\<^sub>t_lam TC have VCS: "?v \<notin> constr_vars (constr_subst ?v (to_unifiable t\<^sub>1) con')" by simp
+  have "htvars (hsubst [?v \<mapsto> to_unifiable t\<^sub>1] e') \<subseteq> 
+    htvars e' - dom [?v \<mapsto> to_unifiable t\<^sub>1] \<union> subst_vars [?v \<mapsto> to_unifiable t\<^sub>1]" 
       by (metis htvars_hsubst)
-  hence "htvars (hsubst [?v \<mapsto> untypeify t\<^sub>1] e') \<subseteq> htvars e' - {?v}" by simp
-  moreover have "htvars (hsubst s (hsubst [?v \<mapsto> untypeify t\<^sub>1] e')) \<subseteq> 
-    htvars (hsubst [?v \<mapsto> untypeify t\<^sub>1] e') - dom s \<union> subst_vars s" by simp
-  ultimately have "htvars (hsubst s (hsubst [?v \<mapsto> untypeify t\<^sub>1] e')) \<subseteq> 
+  hence "htvars (hsubst [?v \<mapsto> to_unifiable t\<^sub>1] e') \<subseteq> htvars e' - {?v}" by simp
+  moreover have "htvars (hsubst s (hsubst [?v \<mapsto> to_unifiable t\<^sub>1] e')) \<subseteq> 
+    htvars (hsubst [?v \<mapsto> to_unifiable t\<^sub>1] e') - dom s \<union> subst_vars s" by simp
+  ultimately have "htvars (hsubst s (hsubst [?v \<mapsto> to_unifiable t\<^sub>1] e')) \<subseteq> 
     htvars e' - {?v} - dom s \<union> subst_vars s" by blast
-  with S have "?v \<notin> htvars (hsubst (extend_subst ?v (untypeify t\<^sub>1) s) e')" by auto
-  with E S VCS have A: "partial_solidify vs (hsubst (extend_subst ?v (untypeify t\<^sub>1) s) e') = 
+  with S have "?v \<notin> htvars (hsubst (extend_subst ?v (to_unifiable t\<^sub>1) s) e')" by auto
+  with E S VCS have A: "partial_solidify vs (hsubst (extend_subst ?v (to_unifiable t\<^sub>1) s) e') = 
     liquify (Lam\<^sub>s x t\<^sub>1 e)" by simp
   from tc\<^sub>t_lam S have U: "?v \<notin> dom s" by auto
-  with S have B: "idempotent (extend_subst ?v (untypeify t\<^sub>1) s)" by simp
-  from S E FV have "s unifies\<^sub>\<kappa> constr_subst ?v (untypeify t\<^sub>1) (partial_typeify_constr vs con)" 
+  with S have B: "idempotent (extend_subst ?v (to_unifiable t\<^sub>1) s)" by simp
+  from S E FV have "s unifies\<^sub>\<kappa> constr_subst ?v (to_unifiable t\<^sub>1) (eliminate_vars_constr vs con)" 
     by simp
-  hence C: "extend_subst ?v (untypeify t\<^sub>1) s unifies\<^sub>\<kappa> partial_typeify_constr vs con" by simp
+  hence C: "extend_subst ?v (to_unifiable t\<^sub>1) s unifies\<^sub>\<kappa> eliminate_vars_constr vs con" by simp
   from E TC have "insert ?v vs \<subseteq> vs'" by (metis vars_expand)
   with tc\<^sub>t_lam have "insert ?v (vs' - insert ?v vs) = vs' - vs" by auto
-  with S E have D: "dom (extend_subst ?v (untypeify t\<^sub>1) s) = vs' - vs" by simp
-  have VS: "uvars (subst s (untypeify t\<^sub>1)) \<subseteq> uvars (untypeify t\<^sub>1) - dom s \<union> subst_vars s" 
+  with S E have D: "dom (extend_subst ?v (to_unifiable t\<^sub>1) s) = vs' - vs" by simp
+  have VS: "uvars (subst s (to_unifiable t\<^sub>1)) \<subseteq> uvars (to_unifiable t\<^sub>1) - dom s \<union> subst_vars s" 
     by (metis uvars_subst)
-  from S U VS have F: "subst_vars (extend_subst ?v (untypeify t\<^sub>1) s) = {}" by auto
-  from S have AR: "partial_typeify (insert ?v vs) 
-    (subst (map_option (subst [fresh vs \<mapsto> untypeify t\<^sub>1]) \<circ> s) 
-    (subst [fresh vs \<mapsto> untypeify t\<^sub>1] t')) = untypeify t\<^sub>2" by (metis subst_absorb_no_ran)
+  from S U VS have F: "subst_vars (extend_subst ?v (to_unifiable t\<^sub>1) s) = {}" by auto
+  from S have AR: "eliminate_vars (insert ?v vs) 
+    (subst (map_option (subst [fresh vs \<mapsto> to_unifiable t\<^sub>1]) \<circ> s) 
+    (subst [fresh vs \<mapsto> to_unifiable t\<^sub>1] t')) = to_unifiable t\<^sub>2" by (metis subst_absorb_no_ran)
   from U have SV: "s ?v = None" by auto
-  have "uvars (subst (extend_subst ?v (untypeify t\<^sub>1) s) t') \<subseteq> 
-    uvars t' - dom (extend_subst ?v (untypeify t\<^sub>1) s) \<union> 
-      subst_vars (extend_subst ?v (untypeify t\<^sub>1) s)" by (metis uvars_subst)
-  with U have "uvars (subst (extend_subst ?v (untypeify t\<^sub>1) s) t') \<subseteq> 
-    uvars t' - insert ?v (dom s) \<union> uvars (subst s (untypeify t\<^sub>1)) \<union> subst_vars s" by simp
+  have "uvars (subst (extend_subst ?v (to_unifiable t\<^sub>1) s) t') \<subseteq> 
+    uvars t' - dom (extend_subst ?v (to_unifiable t\<^sub>1) s) \<union> 
+      subst_vars (extend_subst ?v (to_unifiable t\<^sub>1) s)" by (metis uvars_subst)
+  with U have "uvars (subst (extend_subst ?v (to_unifiable t\<^sub>1) s) t') \<subseteq> 
+    uvars t' - insert ?v (dom s) \<union> uvars (subst s (to_unifiable t\<^sub>1)) \<union> subst_vars s" by simp
   moreover from S have "?v \<notin> 
-    uvars t' - insert ?v (dom s) \<union> uvars (subst s (untypeify t\<^sub>1)) \<union> subst_vars s" by simp
-  ultimately have "?v \<notin> uvars (subst (extend_subst ?v (untypeify t\<^sub>1) s) t')" by auto
-  with E have "?v \<notin> uvars (subst (extend_subst ?v (untypeify t\<^sub>1) s) tt)" by simp
-  with S E AR SV have G: "partial_typeify vs (subst (extend_subst ?v (untypeify t\<^sub>1) s) tt) = 
-    untypeify (Arrow t\<^sub>1 t\<^sub>2)" by (simp add: expand_extend_subst)
-  from S have "valid_ty_subst (extend_subst ?v (untypeify t\<^sub>1) s)" by simp
+    uvars t' - insert ?v (dom s) \<union> uvars (subst s (to_unifiable t\<^sub>1)) \<union> subst_vars s" by simp
+  ultimately have "?v \<notin> uvars (subst (extend_subst ?v (to_unifiable t\<^sub>1) s) t')" by auto
+  with E have "?v \<notin> uvars (subst (extend_subst ?v (to_unifiable t\<^sub>1) s) tt)" by simp
+  with S E AR SV have G: "eliminate_vars vs (subst (extend_subst ?v (to_unifiable t\<^sub>1) s) tt) = 
+    to_unifiable (Arrow t\<^sub>1 t\<^sub>2)" by (simp add: expand_extend_subst)
+  from S have "valid_ty_subst (extend_subst ?v (to_unifiable t\<^sub>1) s)" by simp
   with A B C D F G show ?case by blast
 next
   case (tc\<^sub>t_app e\<^sub>1 t\<^sub>1 t\<^sub>2 e\<^sub>2)
@@ -436,27 +436,27 @@ next
   obtain e\<^sub>2' t\<^sub>2' vs''' con\<^sub>2 where TC2: "typecheck' \<Gamma> vs'' (erase e\<^sub>2) = (e\<^sub>2', t\<^sub>2', vs''', con\<^sub>2)"
     by (metis prod_cases4)
   with tc\<^sub>t_app TC1 have E: "e' = App\<^sub>s e\<^sub>1' e\<^sub>2' \<and> tt = Var ?v \<and> vs''' = vs' \<and> 
-    con = con\<^sub>1 @ con\<^sub>2 @ [(t\<^sub>1', Ctor ''Arrow'' [t\<^sub>2', Var ?v])]" by (auto simp add: Let_def)
+    con = con\<^sub>1 @ con\<^sub>2 @ [(t\<^sub>1', Arrow\<^sub>\<tau> t\<^sub>2' (Var ?v))]" by (auto simp add: Let_def)
   from tc\<^sub>t_app have "subst_vars \<Gamma> \<subseteq> insert ?v vs" by auto
   with tc\<^sub>t_app TC1 obtain s\<^sub>1 where S1: "
     partial_solidify (insert ?v vs) (hsubst s\<^sub>1 e\<^sub>1') = liquify e\<^sub>1 \<and> 
-    partial_typeify (insert ?v vs) (subst s\<^sub>1 t\<^sub>1') = untypeify (Arrow t\<^sub>1 t\<^sub>2) \<and> 
+    eliminate_vars (insert ?v vs) (subst s\<^sub>1 t\<^sub>1') = to_unifiable (Arrow t\<^sub>1 t\<^sub>2) \<and> 
     dom s\<^sub>1 = vs'' - insert ?v vs \<and> subst_vars s\<^sub>1 = {} \<and> 
-    s\<^sub>1 unifies\<^sub>\<kappa> partial_typeify_constr (insert ?v vs) con\<^sub>1 \<and> valid_ty_subst s\<^sub>1 \<and> idempotent s\<^sub>1" 
+    s\<^sub>1 unifies\<^sub>\<kappa> eliminate_vars_constr (insert ?v vs) con\<^sub>1 \<and> valid_ty_subst s\<^sub>1 \<and> idempotent s\<^sub>1" 
       by fastforce
   from TC1 have V1: "insert ?v vs \<subseteq> vs''" by (metis vars_expand)
   from TC2 E have V2: "vs'' \<subseteq> vs'" by (metis vars_expand)
   with tc\<^sub>t_app V1 have Y: "subst_vars \<Gamma> \<subseteq> vs''" by auto
   with tc\<^sub>t_app TC1 TC2 Y obtain s\<^sub>2 where S2: "partial_solidify vs'' (hsubst s\<^sub>2 e\<^sub>2') = liquify e\<^sub>2 \<and> 
-    partial_typeify vs'' (subst s\<^sub>2 t\<^sub>2') = untypeify t\<^sub>1 \<and> dom s\<^sub>2 = vs''' - vs'' \<and> subst_vars s\<^sub>2 = {} \<and> 
-    s\<^sub>2 unifies\<^sub>\<kappa> partial_typeify_constr vs'' con\<^sub>2 \<and> valid_ty_subst s\<^sub>2 \<and> idempotent s\<^sub>2" by fastforce
+    eliminate_vars vs'' (subst s\<^sub>2 t\<^sub>2') = to_unifiable t\<^sub>1 \<and> dom s\<^sub>2 = vs''' - vs'' \<and> subst_vars s\<^sub>2 = {} \<and> 
+    s\<^sub>2 unifies\<^sub>\<kappa> eliminate_vars_constr vs'' con\<^sub>2 \<and> valid_ty_subst s\<^sub>2 \<and> idempotent s\<^sub>2" by fastforce
   from tc\<^sub>t_app have FV: "?v \<notin> vs" by simp
   from S1 S2 have DSS: "dom s\<^sub>1 \<inter> dom s\<^sub>2 = {}" by auto
-  from tc\<^sub>t_app TC1 S1 have "valid_ty_uexpr t\<^sub>1' \<and> valid_ty_subst s\<^sub>1" by auto
-  hence VTS1: "valid_ty_uexpr (subst s\<^sub>1 t\<^sub>1')" by simp
-  from tc\<^sub>t_app TC2 S2 have "valid_ty_uexpr t\<^sub>2' \<and> valid_ty_subst s\<^sub>2" by auto
-  hence VTS2: "valid_ty_uexpr (subst s\<^sub>2 t\<^sub>2')" by simp
-  let ?s = "extend_subst ?v (untypeify t\<^sub>2) (combine_subst s\<^sub>1 s\<^sub>2)"
+  from tc\<^sub>t_app TC1 S1 have "valid_ty_term t\<^sub>1' \<and> valid_ty_subst s\<^sub>1" by auto
+  hence VTS1: "valid_ty_term (subst s\<^sub>1 t\<^sub>1')" by simp
+  from tc\<^sub>t_app TC2 S2 have "valid_ty_term t\<^sub>2' \<and> valid_ty_subst s\<^sub>2" by auto
+  hence VTS2: "valid_ty_term (subst s\<^sub>2 t\<^sub>2')" by simp
+  let ?s = "extend_subst ?v (to_unifiable t\<^sub>2) (combine_subst s\<^sub>1 s\<^sub>2)"
   from S1 have D1: "dom s\<^sub>1 = vs'' - insert ?v vs" by simp
   from S2 E have D2: "dom s\<^sub>2 = vs' - vs''" by simp
   with V1 V2 D1 have D3: "dom (combine_subst s\<^sub>1 s\<^sub>2) = vs' - insert ?v vs" by auto
@@ -474,18 +474,18 @@ next
   with S1 S2 VE1 VE2 HV HVS2 have "partial_solidify vs (hsubst ?s e\<^sub>1') = liquify e\<^sub>1 \<and>
     partial_solidify vs (hsubst ?s e\<^sub>2') = liquify e\<^sub>2" by simp
   hence B: "partial_solidify vs (hsubst ?s (App\<^sub>s e\<^sub>1' e\<^sub>2')) = liquify (App\<^sub>s e\<^sub>1 e\<^sub>2)" by simp
-  have C: "partial_typeify vs (subst ?s (Var ?v)) = untypeify t\<^sub>2" by simp
+  have C: "eliminate_vars vs (subst ?s (Var ?v)) = to_unifiable t\<^sub>2" by simp
   from S1 S2 DSS D3 have D: "subst_vars ?s = {}" by auto
   from S1 S2 have VCS: "?v \<notin> subst_vars s\<^sub>1 \<and> ?v \<notin> subst_vars s\<^sub>2" by auto
   from D2 S1 V1 have D2S1: "dom s\<^sub>2 \<inter> subst_vars s\<^sub>1 = {}" by auto
   from tc\<^sub>t_app TC1 VG have "?v \<notin> constr_vars con\<^sub>1" by simp
-  with S1 S2 DSS D3 D2S1 have UC1: "?s unifies\<^sub>\<kappa> partial_typeify_constr vs con\<^sub>1" by simp
+  with S1 S2 DSS D3 D2S1 have UC1: "?s unifies\<^sub>\<kappa> eliminate_vars_constr vs con\<^sub>1" by simp
   from V1 V2 have VVS': "vs \<subseteq> vs''" by simp
   from tc\<^sub>t_app TC1 TC2 E have "constr_vars con\<^sub>2 \<subseteq> vs' - vs'' \<union> subst_vars \<Gamma>" by simp
   with tc\<^sub>t_app have "constr_vars con\<^sub>2 \<inter> vs'' \<subseteq> vs" by auto
-  with S2 VVS' have "s\<^sub>2 unifies\<^sub>\<kappa> partial_typeify_constr vs con\<^sub>2" 
+  with S2 VVS' have "s\<^sub>2 unifies\<^sub>\<kappa> eliminate_vars_constr vs con\<^sub>2" 
     by (metis partial_typeify_constr_reduce_subset)
-  with S1 S2 DSS D3 have UC2: "?s unifies\<^sub>\<kappa> partial_typeify_constr vs con\<^sub>2" by simp
+  with S1 S2 DSS D3 have UC2: "?s unifies\<^sub>\<kappa> eliminate_vars_constr vs con\<^sub>2" by simp
   from tc\<^sub>t_app TC1 have UV1: "uvars t\<^sub>1' \<subseteq> vs'' - insert ?v vs \<union> subst_vars \<Gamma>" by simp
   with VG have VT1: "?v \<notin> uvars t\<^sub>1'" by auto
   from tc\<^sub>t_app D2 V1 UV1 have DU1: "dom s\<^sub>2 \<inter> uvars t\<^sub>1' = {}" by auto
@@ -509,39 +509,37 @@ next
   with D1 US2 have DU2: "dom s\<^sub>1 \<inter> uvars (subst s\<^sub>2 t\<^sub>2') = {}" by fast
   from D1 have DSV1: "dom s\<^sub>1 \<inter> vs = {}" by auto
   from D2 V1 have DSV2: "dom s\<^sub>2 \<inter> vs = {}" by auto
-  from S1 obtain tt1 tt2 where SS1: "subst s\<^sub>1 t\<^sub>1' = Ctor ''Arrow'' [tt1, tt2] \<and> 
-    partial_typeify (insert ?v vs) tt1 = untypeify t\<^sub>1 \<and> 
-    partial_typeify (insert ?v vs) tt2 = untypeify t\<^sub>2" by auto
+  from S1 obtain tt1 tt2 where SS1: "subst s\<^sub>1 t\<^sub>1' = Arrow\<^sub>\<tau> tt1 tt2 \<and> 
+    eliminate_vars (insert ?v vs) tt1 = to_unifiable t\<^sub>1 \<and> 
+    eliminate_vars (insert ?v vs) tt2 = to_unifiable t\<^sub>2" by auto
   from US1 SS1 have "uvars tt1 \<subseteq> vs \<and> uvars tt2 \<subseteq> vs" by simp
-  with FV SS1 have PT1: "partial_typeify vs tt1 = untypeify t\<^sub>1 \<and> 
-    partial_typeify vs tt2 = untypeify t\<^sub>2" by force
+  with FV SS1 have PT1: "eliminate_vars vs tt1 = to_unifiable t\<^sub>1 \<and> 
+    eliminate_vars vs tt2 = to_unifiable t\<^sub>2" by force
   from US2 have "uvars (subst s\<^sub>2 t\<^sub>2') \<inter> vs'' \<subseteq> vs" by auto
-  with S2 VVS' have "partial_typeify vs (subst s\<^sub>2 t\<^sub>2') = untypeify t\<^sub>1"
+  with S2 VVS' have "eliminate_vars vs (subst s\<^sub>2 t\<^sub>2') = to_unifiable t\<^sub>1"
     by (metis partial_typeify_reduce_subset)
   with FV UC1 UC2 S1 S2 DSV1 DSV2 VT1 VT2 DU1 DU2 SS1 PT1 have F: "
-    ?s unifies\<^sub>\<kappa> partial_typeify_constr vs (con\<^sub>1 @ con\<^sub>2 @ [(t\<^sub>1', Ctor ''Arrow'' [t\<^sub>2', Var ?v])])" 
+    ?s unifies\<^sub>\<kappa> eliminate_vars_constr vs (con\<^sub>1 @ con\<^sub>2 @ [(t\<^sub>1', Arrow\<^sub>\<tau> t\<^sub>2' (Var ?v))])" 
       by (simp add: expand_extend_subst)
   from DSS VCS V1 D1 D2 S1 S2 D2S1 have G: "idempotent ?s" by simp
   from S1 S2 have "valid_ty_subst ?s" by simp
   with E A B C D F G show ?case by blast
 qed auto
 
-lemma typecheck_fails [simp]: "typecheck e = None \<Longrightarrow> 
-  \<nexists>e\<^sub>t t. (Map.empty \<turnstile>\<^sub>t e\<^sub>t : t) \<and> tvarst e\<^sub>t = {} \<and> e = erase e\<^sub>t"
+lemma typecheck_fails [simp]: "typecheck e = None \<Longrightarrow> \<nexists>e\<^sub>t t. (Map.empty \<turnstile>\<^sub>t e\<^sub>t : t) \<and> e = erase e\<^sub>t"
 proof                              
   assume "typecheck e = None"
   then obtain e' tt vs' con where X: "typecheck' Map.empty {} e = (e', tt, vs', con) \<and> 
     unify con = None" by (auto split: prod.splits option.splits)
-  assume "\<exists>e\<^sub>t t. (Map.empty \<turnstile>\<^sub>t e\<^sub>t : t) \<and> tvarst e\<^sub>t = {} \<and> e = erase e\<^sub>t"
-  then obtain e\<^sub>t t where Y: "(map_option typeify \<circ> Map.empty \<turnstile>\<^sub>t e\<^sub>t : t) \<and> tvarst e\<^sub>t = {} \<and> 
-    e = erase e\<^sub>t" by fastforce
+  assume "\<exists>e\<^sub>t t. (Map.empty \<turnstile>\<^sub>t e\<^sub>t : t) \<and> e = erase e\<^sub>t"
+  then obtain e\<^sub>t t where Y: "(map_option to_type \<circ> Map.empty \<turnstile>\<^sub>t e\<^sub>t : t) \<and> e = erase e\<^sub>t" by fastforce
   have Z: "subst_vars Map.empty \<subseteq> {}" by simp
   have "valid_ty_subst Map.empty \<and> finite {}" by simp
   with X Y Z have "\<exists>s. partial_solidify {} (hsubst s e') = liquify e\<^sub>t \<and> 
-    partial_typeify {} (subst s tt) = untypeify t \<and> dom s = vs' - {} \<and> subst_vars s = {} \<and> 
-    s unifies\<^sub>\<kappa> partial_typeify_constr {} con \<and> valid_ty_subst s \<and> idempotent s" 
+    eliminate_vars {} (subst s tt) = to_unifiable t \<and> dom s = vs' - {} \<and> subst_vars s = {} \<and> 
+    s unifies\<^sub>\<kappa> eliminate_vars_constr {} con \<and> valid_ty_subst s \<and> idempotent s" 
     using typecheck_fails' by blast
-  then obtain s where "s unifies\<^sub>\<kappa> partial_typeify_constr {} con \<and> idempotent s" by blast
+  then obtain s where "s unifies\<^sub>\<kappa> eliminate_vars_constr {} con \<and> idempotent s" by blast
   hence "\<exists>s'. unify con = Some s' \<and> s specializes s'" by simp
   with X show "False" by simp
 qed
