02Typed/UnifiableType.thy
@@ -2,221 +2,186 @@ theory UnifiableType
   imports Type "../00Utils/Unification/Unification"
 begin
 
-definition env_subst :: "subst \<Rightarrow> subst \<Rightarrow> subst" where
-  "env_subst sub \<Gamma> \<equiv> map_option (subst sub) \<circ> \<Gamma>"
+subsection \<open>Unifiable Types\<close>
 
-fun typeify :: "uterm \<Rightarrow> ty" where
-  "typeify (Var v) = Num"
-| "typeify (Ctor \<gamma> []) = (if \<gamma> = ''Num'' then Num else undefined)"
-| "typeify (Ctor \<gamma> [\<tau>\<^sub>1, \<tau>\<^sub>2]) = 
-    (if \<gamma> = ''Arrow'' then Arrow (typeify \<tau>\<^sub>1) (typeify \<tau>\<^sub>2) else undefined)"
-| "typeify (Ctor \<gamma> \<tau>s) = undefined"
+text \<open>Before we can define the typechecking algorithm itself, we need to define a conversion between
+our actual types and unifiable terms.\<close>
 
-primrec untypeify :: "ty \<Rightarrow> uterm" where
-  "untypeify Num = Ctor ''Num'' []"
-| "untypeify (Arrow t\<^sub>1 t\<^sub>2) = Ctor ''Arrow'' [untypeify t\<^sub>1, untypeify t\<^sub>2]"
+abbreviation Num\<^sub>\<tau> :: "uterm" where
+  "Num\<^sub>\<tau> \<equiv> Ctor ''Num'' []"
 
-definition partial_typeify :: "var set \<Rightarrow> uterm \<Rightarrow> uterm" where
-  "partial_typeify vs t \<equiv> subst (\<lambda>x. if x \<in> vs then Some (Ctor ''Num'' []) else None) t"
+abbreviation Arrow\<^sub>\<tau> :: "uterm \<Rightarrow> uterm \<Rightarrow> uterm" where
+  "Arrow\<^sub>\<tau> \<tau>\<^sub>1 \<tau>\<^sub>2 \<equiv> Ctor ''Arrow'' [\<tau>\<^sub>1, \<tau>\<^sub>2]"
 
-abbreviation partial_typeify_constr :: "var set \<Rightarrow> constraint \<Rightarrow> constraint" where
-  "partial_typeify_constr vs k \<equiv> map (\<lambda>(e1, e2). (partial_typeify vs e1, partial_typeify vs e2)) k"
+primrec to_unifiable :: "ty \<Rightarrow> uterm" where
+  "to_unifiable Num = Num\<^sub>\<tau>"
+| "to_unifiable (Arrow t\<^sub>1 t\<^sub>2) = Arrow\<^sub>\<tau> (to_unifiable t\<^sub>1) (to_unifiable t\<^sub>2)"
 
-fun valid_ty_uexpr' :: "string \<Rightarrow> nat \<Rightarrow> bool" where
-  "valid_ty_uexpr' \<gamma> 0 = (\<gamma> = ''Num'')"
-| "valid_ty_uexpr' \<gamma> (Suc 0) = False"
-| "valid_ty_uexpr' \<gamma> (Suc (Suc 0)) = (\<gamma> = ''Arrow'')"
-| "valid_ty_uexpr' \<gamma> (Suc (Suc (Suc x))) = False"
+lemma uvars_of_type [simp]: "uvars (to_unifiable t) = {}"
+  by (induction t) simp_all
 
-primrec valid_ty_uexpr :: "uterm \<Rightarrow> bool" where
-  "valid_ty_uexpr (Var v) = True"
-| "valid_ty_uexpr (Ctor \<gamma> \<tau>s) = (valid_ty_uexpr' \<gamma> (length \<tau>s) \<and> list_all valid_ty_uexpr \<tau>s)"
+text \<open>The reverse direction presents some complications. Not every term corresponds to a type; we 
+can solve this simply enough with a well-formedness condition \<open>valid_ty_uexpr\<close>. More subtly, a term 
+may contain free variables, and a type cannot. We map all term variables, arbitrarily, to the \<open>Num\<close> 
+type. Any choice would do as well, of course, but the fact that we have had to make a choice at all 
+will lead to some properties becoming more complicated down the line.\<close>
 
-definition valid_ty_uexprs :: "constraint \<Rightarrow> bool" where
-  "valid_ty_uexprs \<tau>s = list_all (\<lambda>(\<tau>\<^sub>1, \<tau>\<^sub>2). valid_ty_uexpr \<tau>\<^sub>1 \<and> valid_ty_uexpr \<tau>\<^sub>2) \<tau>s"
- 
+fun to_type :: "uterm \<Rightarrow> ty" where
+  "to_type (Var v) = Num"
+| "to_type (Ctor \<gamma> []) = (if \<gamma> = ''Num'' then Num else undefined)"
+| "to_type (Ctor \<gamma> [\<tau>\<^sub>1, \<tau>\<^sub>2]) = 
+    (if \<gamma> = ''Arrow'' then Arrow (to_type \<tau>\<^sub>1) (to_type \<tau>\<^sub>2) else undefined)"
+| "to_type (Ctor \<gamma> \<tau>s) = undefined"
+
+fun valid_ty_term' :: "string \<Rightarrow> nat \<Rightarrow> bool" where
+  "valid_ty_term' \<gamma> 0 = (\<gamma> = ''Num'')"
+| "valid_ty_term' \<gamma> (Suc 0) = False"
+| "valid_ty_term' \<gamma> (Suc (Suc 0)) = (\<gamma> = ''Arrow'')"
+| "valid_ty_term' \<gamma> (Suc (Suc (Suc x))) = False"
+
+primrec valid_ty_term :: "uterm \<Rightarrow> bool" where
+  "valid_ty_term (Var v) = True"
+| "valid_ty_term (Ctor \<gamma> \<tau>s) = (valid_ty_term' \<gamma> (length \<tau>s) \<and> list_all valid_ty_term \<tau>s)"
+
+lemma to_unif_to_type [simp]: "to_type (to_unifiable t) = t"
+  by (induction t) simp_all
+
+lemma to_type_to_unif [simp]: "valid_ty_term \<tau> \<Longrightarrow> uvars \<tau> = {} \<Longrightarrow> to_unifiable (to_type \<tau>) = \<tau>"
+  by (induction \<tau> rule: to_type.induct) simp_all
+
+lemma to_unifiable_valid [simp]: "valid_ty_term (to_unifiable t)"
+  by (induction t) simp_all
+
+text \<open>We extend our well-formedness condition to substitutions in the obvious way:\<close>
+
 definition valid_ty_subst :: "subst \<Rightarrow> bool" where
-  "valid_ty_subst \<Gamma> = (\<forall>\<tau> \<in> ran \<Gamma>. valid_ty_uexpr \<tau>)"
+  "valid_ty_subst \<sigma> \<equiv> (\<forall>\<tau> \<in> ran \<sigma>. valid_ty_term \<tau>)"
 
-lemma [simp]: "typeify (untypeify t) = t"
-  by (induction t) simp_all
+lemma valid_empty_subst [simp]: "valid_ty_subst Map.empty"
+  by (simp add: valid_ty_subst_def)
 
-lemma [simp]: "valid_ty_uexpr t \<Longrightarrow> uvars t = {} \<Longrightarrow> untypeify (typeify t) = t"
-  by (induction t rule: typeify.induct) simp_all
-
-lemma [dest]: "typeify e = Arrow t\<^sub>1 t\<^sub>2 \<Longrightarrow> valid_ty_uexpr e \<Longrightarrow> uvars e = {} \<Longrightarrow> 
-    e = Ctor ''Arrow'' [untypeify t\<^sub>1, untypeify t\<^sub>2]"
-  by (induction e rule: typeify.induct) auto
-
-lemma [simp]: "uvars (untypeify t) = {}"
-  by (induction t) simp_all
-
-lemma [simp]: "valid_ty_uexpr (untypeify t)"
-  by (induction t) simp_all
-
-lemma [simp]: "partial_typeify {} t = t"
-  by (simp add: partial_typeify_def)
-
-lemma [simp]: "x \<notin> uvars t \<Longrightarrow> partial_typeify (insert x vs) t = partial_typeify vs t"
-  and "x \<notin> uvarss ts \<Longrightarrow> map (partial_typeify (insert x vs)) ts = map (partial_typeify vs) ts"
-  by (induction t and ts rule: uvars_uvarss.induct) (simp_all add: partial_typeify_def)
-
-lemma partial_typeify_reduce_subset: "uvars t \<inter> vs' \<subseteq> vs \<Longrightarrow> vs \<subseteq> vs' \<Longrightarrow>
-    partial_typeify vs' t = partial_typeify vs t"
-  and "uvarss ts \<inter> vs' \<subseteq> vs \<Longrightarrow> vs \<subseteq> vs' \<Longrightarrow>
-    map (partial_typeify vs') ts = map (partial_typeify vs) ts"
-proof (induction t and ts rule: uvars_uvarss.induct)
-  case (4 \<tau> \<tau>s)
-  moreover hence "uvars \<tau> \<inter> vs' \<subseteq> vs \<and> uvarss \<tau>s \<inter> vs' \<subseteq> vs" by auto
-  ultimately show ?case by simp
-qed (auto simp add: partial_typeify_def)
-
-lemma [simp]: "partial_typeify vs (untypeify t) = untypeify t"
-  by (induction t) (simp_all add: partial_typeify_def)
-
-lemma [simp]: "partial_typeify vs (Var x) = (if x \<in> vs then Ctor ''Num'' [] else Var x)"
-  by (simp add: partial_typeify_def)
-
-lemma [simp]: "partial_typeify vs (Ctor \<gamma> ts) = Ctor \<gamma> (map (partial_typeify vs) ts)"
-  by (simp add: partial_typeify_def)
-
-lemma [simp]: "uvars t \<subseteq> vs \<Longrightarrow> valid_ty_uexpr t \<Longrightarrow> partial_typeify vs t = untypeify (typeify t)"
-  by (induction t rule: typeify.induct) (simp_all add: partial_typeify_def)
-
-lemma [simp]: "uvars t = {} \<Longrightarrow> partial_typeify vs t = t"
-  and "uvarss ts = {} \<Longrightarrow> map (partial_typeify vs) ts = ts"
-  by (induction t and ts rule: uvars_uvarss.induct) simp_all
-
-lemma [elim]: "valid_ty_subst \<Gamma> \<Longrightarrow> \<Gamma> x = Some t \<Longrightarrow> valid_ty_uexpr t"
+lemma valid_upd_subst [simp]: "valid_ty_subst \<sigma> \<Longrightarrow> valid_ty_term \<tau> \<Longrightarrow> valid_ty_subst (\<sigma>(x \<mapsto> \<tau>))"
   by (auto simp add: valid_ty_subst_def ran_def)
 
-lemma [simp]: "subst_vars \<Gamma> \<subseteq> vs \<Longrightarrow> valid_ty_subst \<Gamma> \<Longrightarrow> \<Gamma> x = Some t \<Longrightarrow> 
-    partial_typeify vs t = untypeify (typeify t)"
+lemma valid_term_from_subst [elim]: "valid_ty_subst \<sigma> \<Longrightarrow> \<sigma> x = Some \<tau> \<Longrightarrow> valid_ty_term \<tau>"
+  by (auto simp add: valid_ty_subst_def ran_def)
+
+lemma valid_substituted_term [simp]: "valid_ty_term \<tau> \<Longrightarrow> valid_ty_subst \<sigma> \<Longrightarrow> 
+    valid_ty_term (subst \<sigma> \<tau>)"
+  and "list_all valid_ty_term \<tau>s \<Longrightarrow> valid_ty_subst \<sigma> \<Longrightarrow> 
+    list_all valid_ty_term (map (subst \<sigma>) \<tau>s)"
+  by (induction \<tau> and \<tau>s rule: uvars_uvarss.induct) 
+     (auto simp add: valid_ty_subst_def ran_def split: option.splits)
+
+lemma valid_extend_subst [simp]: "valid_ty_subst \<sigma> \<Longrightarrow> valid_ty_term \<tau> \<Longrightarrow> 
+    valid_ty_subst (extend_subst x \<tau> \<sigma>)"
+  by (auto simp add: valid_ty_subst_def extend_subst_def ran_def)
+
+lemma valid_combine_subst [simp]: "valid_ty_subst \<sigma>\<^sub>1 \<Longrightarrow> valid_ty_subst \<sigma>\<^sub>2 \<Longrightarrow> 
+  valid_ty_subst (combine_subst \<sigma>\<^sub>1 \<sigma>\<^sub>2)"
+proof (unfold valid_ty_subst_def combine_subst_def ran_def, rule)
+  fix \<tau>
+  assume S1: "\<forall>\<tau>' \<in> {\<tau>''. \<exists>x. \<sigma>\<^sub>1 x = Some \<tau>''}. valid_ty_term \<tau>'"
+  assume S2: "\<forall>\<tau>' \<in> {\<tau>''. \<exists>x. \<sigma>\<^sub>2 x = Some \<tau>''}. valid_ty_term \<tau>'"
+  assume "\<tau> \<in> {\<tau>''. \<exists>x. (case \<sigma>\<^sub>2 x of None \<Rightarrow> \<sigma>\<^sub>1 x | Some \<tau>' \<Rightarrow> Some (subst \<sigma>\<^sub>1 \<tau>')) = Some \<tau>''}"
+  then obtain x where X: "(case \<sigma>\<^sub>2 x of None \<Rightarrow> \<sigma>\<^sub>1 x | Some \<tau>' \<Rightarrow> Some (subst \<sigma>\<^sub>1 \<tau>')) = Some \<tau>" 
+    by auto
+  from S1 S2 X show "valid_ty_term \<tau>" 
+  proof (cases "\<sigma>\<^sub>2 x")
+    case (Some \<tau>')
+    from S1 have "valid_ty_subst \<sigma>\<^sub>1" by (auto simp add: valid_ty_subst_def ran_def)
+    with S2 X Some show ?thesis by auto
+  qed auto
+qed
+
+text \<open>Now on to the promised complications. Because the types we produce are not the fully-general 
+ones produced by the unification algorithm, we need an operation to replace term variables with 
+\<open>Num\<^sub>\<tau>\<close>s. But we still may need to instantiate some of them, to extend a subexpression type 
+reconstruction to a larger expression. So we provide a set of variables to eliminate:\<close>
+
+definition eliminate_vars :: "var set \<Rightarrow> uterm \<Rightarrow> uterm" where
+  "eliminate_vars vs \<equiv> subst (\<lambda>x. if x \<in> vs then Some Num\<^sub>\<tau> else None)"
+
+lemma eliminate_no_vars [simp]: "eliminate_vars {} \<tau> = \<tau>"
+  by (simp add: eliminate_vars_def)
+
+lemma eliminate_unused_var [simp]: "x \<notin> uvars \<tau> \<Longrightarrow> 
+    eliminate_vars (insert x vs) \<tau> = eliminate_vars vs \<tau>"
+  and "x \<notin> uvarss \<tau>s \<Longrightarrow> map (eliminate_vars (insert x vs)) \<tau>s = map (eliminate_vars vs) \<tau>s"
+  by (induction \<tau> and \<tau>s rule: uvars_uvarss.induct) (simp_all add: eliminate_vars_def)
+
+lemma eliminate_all_vars [simp]: "uvars \<tau> \<subseteq> vs \<Longrightarrow> valid_ty_term \<tau> \<Longrightarrow> 
+    eliminate_vars vs \<tau> = to_unifiable (to_type \<tau>)"
+  by (induction \<tau> rule: to_type.induct) (simp_all add: eliminate_vars_def)
+
+lemma eliminate_all_vars_ran [simp]: "subst_vars \<sigma> \<subseteq> vs \<Longrightarrow> valid_ty_subst \<sigma> \<Longrightarrow> \<sigma> x = Some \<tau> \<Longrightarrow> 
+    eliminate_vars vs \<tau> = to_unifiable (to_type \<tau>)"
 proof -
-  assume "valid_ty_subst \<Gamma>" and T: "\<Gamma> x = Some t"
-  hence X: "valid_ty_uexpr t" by auto
-  assume "subst_vars \<Gamma> \<subseteq> vs" 
-  with T have "uvars t \<subseteq> vs" by auto
+  assume "valid_ty_subst \<sigma>" and T: "\<sigma> x = Some \<tau>"
+  hence X: "valid_ty_term \<tau>" by auto
+  assume "subst_vars \<sigma> \<subseteq> vs" 
+  with T have "uvars \<tau> \<subseteq> vs" by auto
   with X show ?thesis by simp
 qed
 
-lemma [dest]: "partial_typeify vs t = Ctor ''Arrow'' [t\<^sub>1, t\<^sub>2] \<Longrightarrow> \<exists>tt1 tt2. 
-    t = Ctor ''Arrow'' [tt1, tt2] \<and> partial_typeify vs tt1 = t\<^sub>1 \<and> partial_typeify vs tt2 = t\<^sub>2"
-  by (induction t) (auto simp add: partial_typeify_def split: if_splits)
+lemma eliminate_vars_simp_var [simp]: "eliminate_vars vs (Var x) = (if x \<in> vs then Num\<^sub>\<tau> else Var x)"
+  by (simp add: eliminate_vars_def)
 
-lemma [simp]: "dom s \<inter> vs = {} \<Longrightarrow> subst_vars s = {} \<Longrightarrow> 
-  subst s (partial_typeify vs t) = partial_typeify vs (subst s t)"
-proof (induction t)
+lemma eliminate_vars_simp_ctor [simp]: "eliminate_vars vs (Ctor \<gamma> \<tau>s) = 
+    Ctor \<gamma> (map (eliminate_vars vs) \<tau>s)"
+  by (simp add: eliminate_vars_def)
+
+lemma eliminate_vars_to_arrow [dest]: "eliminate_vars vs \<tau> = Arrow\<^sub>\<tau> \<tau>\<^sub>1 \<tau>\<^sub>2 \<Longrightarrow> \<exists>\<tau>\<^sub>1' \<tau>\<^sub>2'. 
+    \<tau> = Arrow\<^sub>\<tau> \<tau>\<^sub>1' \<tau>\<^sub>2' \<and> eliminate_vars vs \<tau>\<^sub>1' = \<tau>\<^sub>1 \<and> eliminate_vars vs \<tau>\<^sub>2' = \<tau>\<^sub>2"
+  by (induction \<tau>) (auto simp add: eliminate_vars_def split: if_splits)
+
+lemma eliminate_vars_closed [simp]: "uvars \<tau> = {} \<Longrightarrow> eliminate_vars vs \<tau> = \<tau>"
+  and "uvarss \<tau>s = {} \<Longrightarrow> map (eliminate_vars vs) \<tau>s = \<tau>s"
+  by (induction \<tau> and \<tau>s rule: uvars_uvarss.induct) simp_all
+
+lemma subst_eliminate_vars [simp]: "dom \<sigma> \<inter> vs = {} \<Longrightarrow> subst_vars \<sigma> = {} \<Longrightarrow> 
+  subst \<sigma> (eliminate_vars vs \<tau>) = eliminate_vars vs (subst \<sigma> \<tau>)"
+proof (induction \<tau>)
   case (Var x)
   thus ?case
-  proof (cases "s x")
+  proof (cases "\<sigma> x")
     case (Some \<tau>)
     moreover with Var have "uvars \<tau> = {}" by (auto simp add: subst_vars_def ran_def)
     moreover from Var Some have "x \<notin> vs" by auto
     ultimately show ?thesis by simp
-  qed (simp_all add: partial_typeify_def)
+  qed (simp_all add: eliminate_vars_def)
 qed simp_all
 
-lemma [simp]: "x \<notin> constr_vars k \<Longrightarrow> 
-    partial_typeify_constr (insert x vs) k = partial_typeify_constr vs k"
-  by (induction k rule: constr_vars.induct) simp_all
+lemma partial_typeify_reduce_subset: "uvars \<tau> \<inter> vs' \<subseteq> vs \<Longrightarrow> vs \<subseteq> vs' \<Longrightarrow>
+    eliminate_vars vs' \<tau> = eliminate_vars vs \<tau>"
+  and "uvarss \<tau>s \<inter> vs' \<subseteq> vs \<Longrightarrow> vs \<subseteq> vs' \<Longrightarrow>
+    map (eliminate_vars vs') \<tau>s = map (eliminate_vars vs) \<tau>s"
+proof (induction \<tau> and \<tau>s rule: uvars_uvarss.induct)
+  case (4 \<tau> \<tau>s)
+  moreover hence "uvars \<tau> \<inter> vs' \<subseteq> vs \<and> uvarss \<tau>s \<inter> vs' \<subseteq> vs" by auto
+  ultimately show ?case by simp
+qed (auto simp add: eliminate_vars_def)
 
-lemma [simp]: "x \<notin> vs \<Longrightarrow> constr_subst x (untypeify t) (partial_typeify_constr vs con) = 
-    partial_typeify_constr vs (constr_subst x (untypeify t) con)"
-  by (induction x "untypeify t" con rule: constr_subst.induct) simp_all
+text \<open>Again, we extend in the obvious way to constraints.\<close>
 
-lemma partial_typeify_constr_reduce_subset: "constr_vars con \<inter> vs' \<subseteq> vs \<Longrightarrow> vs \<subseteq> vs' \<Longrightarrow>
-    partial_typeify_constr vs' con = partial_typeify_constr vs con"
-proof (induction con rule: constr_subst.induct)
+abbreviation eliminate_vars_constr :: "var set \<Rightarrow> constraint \<Rightarrow> constraint" where
+  "eliminate_vars_constr vs \<equiv> map (\<lambda>(\<tau>\<^sub>1, \<tau>\<^sub>2). (eliminate_vars vs \<tau>\<^sub>1, eliminate_vars vs \<tau>\<^sub>2))"
+
+lemma eliminate_unused_var_constr [simp]: "x \<notin> constr_vars \<kappa> \<Longrightarrow> 
+    eliminate_vars_constr (insert x vs) \<kappa> = eliminate_vars_constr vs \<kappa>"
+  by (induction \<kappa> rule: constr_vars.induct) simp_all
+
+lemma constr_subst_eliminate_vars [simp]: "x \<notin> vs \<Longrightarrow>
+  constr_subst x (to_unifiable \<tau>) (eliminate_vars_constr vs \<kappa>) = 
+    eliminate_vars_constr vs (constr_subst x (to_unifiable \<tau>) \<kappa>)"
+  by (induction x "to_unifiable \<tau>" \<kappa> rule: constr_subst.induct) simp_all
+
+lemma partial_typeify_constr_reduce_subset: "constr_vars \<kappa> \<inter> vs' \<subseteq> vs \<Longrightarrow> vs \<subseteq> vs' \<Longrightarrow>
+    eliminate_vars_constr vs' \<kappa> = eliminate_vars_constr vs \<kappa>"
+proof (induction \<kappa> rule: constr_subst.induct)
   case (2 x \<tau> \<tau>\<^sub>1 \<tau>\<^sub>2 \<kappa>)
   moreover hence "constr_vars \<kappa> \<inter> vs' \<subseteq> vs \<and> uvars \<tau>\<^sub>1 \<inter> vs' \<subseteq> vs \<and> uvars \<tau>\<^sub>2 \<inter> vs' \<subseteq> vs" by auto
   ultimately show ?case by (simp add: partial_typeify_reduce_subset)
 qed simp_all
-
-lemma valid_empty [simp]: "valid_ty_subst Map.empty"
-  by (simp add: valid_ty_subst_def)
-
-lemma [simp]: "valid_ty_subst \<Gamma> \<Longrightarrow> valid_ty_uexpr t \<Longrightarrow> valid_ty_subst (\<Gamma>(x \<mapsto> t))"
-  by (auto simp add: valid_ty_subst_def ran_def)
-
-lemma [simp]: "valid_ty_subst \<Gamma> \<Longrightarrow> valid_ty_subst \<Gamma>' \<Longrightarrow> valid_ty_subst (\<Gamma>(x := \<Gamma>' y))"
-  by (auto simp add: valid_ty_subst_def ran_def)
-
-lemma [simp]: "valid_ty_uexpr e \<Longrightarrow> valid_ty_uexpr e' \<Longrightarrow> valid_ty_uexpr (subst [x \<mapsto> e'] e)"
-  and [simp]: "list_all valid_ty_uexpr es \<Longrightarrow> valid_ty_uexpr e' \<Longrightarrow> 
-    list_all valid_ty_uexpr (map (subst [x \<mapsto> e']) es)"
-proof (induction e and es rule: uvars_uvarss.induct)
-  case (2 k es)
-  thus ?case 
-  proof (induction es)
-    case (Cons a es)
-    thus ?case 
-    proof (induction es)
-      case (Cons b es)
-      thus ?case by (induction es) simp_all
-    qed simp_all
-  qed simp_all
-qed simp_all
-
-lemma [simp]: "valid_ty_uexpr e \<Longrightarrow> valid_ty_uexprs ess \<Longrightarrow> valid_ty_uexprs (constr_subst x e ess)"
-  by (induction ess rule: constr_subst.induct) (auto simp add: valid_ty_uexprs_def)
-
-lemma [simp]: "valid_ty_uexpr t \<Longrightarrow> valid_ty_subst sub \<Longrightarrow> valid_ty_uexpr (subst sub t)"
-  and [simp]: "list_all valid_ty_uexpr ts \<Longrightarrow> valid_ty_subst sub \<Longrightarrow> 
-    list_all valid_ty_uexpr (map (subst sub) ts)"
-  by (induction t and ts rule: uvars_uvarss.induct) 
-     (auto simp add: valid_ty_subst_def ran_def split: option.splits)
-
-lemma [simp]: "valid_ty_subst s \<Longrightarrow> valid_ty_uexpr e \<Longrightarrow> valid_ty_subst (extend_subst x e s)"
-  by (auto simp add: valid_ty_subst_def extend_subst_def ran_def)
-
-lemma [elim]: "valid_ty_uexprs ts \<Longrightarrow> unify ts = Some sub \<Longrightarrow> valid_ty_subst sub"                                  
-proof (induction ts arbitrary: sub rule: unify.induct)
-  case (2 k\<^sub>1 es\<^sub>1 k\<^sub>2 es\<^sub>2 ess)
-  moreover hence "list_all valid_ty_uexpr es\<^sub>1" by (auto simp add: valid_ty_uexprs_def)
-  moreover from 2 have "list_all valid_ty_uexpr es\<^sub>2" by (auto simp add: valid_ty_uexprs_def)
-  ultimately show ?case by (simp add: valid_ty_uexprs_def split: if_splits)
-next
-  case (4 x e ess)
-  thus ?case
-  proof (cases "e = Var x")
-    case False note F = False
-    with 4 show ?thesis 
-    proof (cases "x \<in> uvars e")
-      case False
-      with 4 F obtain sub' where S: "unify (constr_subst x e ess) = Some sub' \<and> 
-        sub = extend_subst x e sub'" by auto
-      from 4 have "valid_ty_uexpr e \<and> valid_ty_uexprs ess" by (simp add: valid_ty_uexprs_def)
-      hence "valid_ty_uexprs (constr_subst x e ess)" by simp
-      with 4 F False S show ?thesis by (simp add: valid_ty_uexprs_def)
-    qed simp_all
-  qed (simp_all add: valid_ty_uexprs_def)
-qed (auto simp add: valid_ty_uexprs_def)
-
-lemma valid_ty_uexpr_structrual [simp]: "structural valid_ty_uexpr"
-  by (auto simp add: structural_def)
-
-lemma [simp]: "valid_ty_subst sub \<Longrightarrow> valid_ty_subst \<Gamma> \<Longrightarrow> valid_ty_subst (env_subst sub \<Gamma>)"
-  by (auto simp add: valid_ty_subst_def env_subst_def ran_def)
-
-lemma [simp]: "valid_ty_subst s1 \<Longrightarrow> valid_ty_subst s2 \<Longrightarrow> valid_ty_subst (combine_subst s1 s2)"
-proof (unfold valid_ty_subst_def combine_subst_def ran_def, rule)
-  fix x
-  assume S1: "\<forall>x \<in> {b. \<exists>a. s1 a = Some b}. valid_ty_uexpr x"
-  assume S2: "\<forall>x \<in> {b. \<exists>a. s2 a = Some b}. valid_ty_uexpr x"
-  assume "x \<in> {b. \<exists>a. (case s2 a of None \<Rightarrow> s1 a | Some e \<Rightarrow> Some (subst s1 e)) = Some b}"
-  then obtain y where Y: "(case s2 y of None \<Rightarrow> s1 y | Some e \<Rightarrow> Some (subst s1 e)) = Some x" 
-    by auto
-  from S1 S2 Y show "valid_ty_uexpr x" 
-  proof (cases "s2 y")
-    case (Some e)
-    from S1 have "valid_ty_subst s1" by (auto simp add: valid_ty_subst_def ran_def)
-    with S2 Y Some show ?thesis by auto
-  qed auto
-qed
-
-lemma [dest]: "typeify \<tau> = Arrow t\<^sub>1 t\<^sub>2 \<Longrightarrow> valid_ty_uexpr \<tau> \<Longrightarrow>
-    \<exists>\<tau>\<^sub>1 \<tau>\<^sub>2. \<tau> = Ctor ''Arrow'' [\<tau>\<^sub>1, \<tau>\<^sub>2] \<and> typeify \<tau>\<^sub>1 = t\<^sub>1 \<and> typeify \<tau>\<^sub>2 = t\<^sub>2"
-  by (induction \<tau> rule: typeify.induct) simp_all
 
 end
